ocaml/ast.ml
@@ -26,6 +26,7 @@ type named_param = {
 type named_fn_def = {
   nf_name           : name;
   nf_lifetime_names : string list;
+  nf_outlives       : (TypeChecker.lifetime * TypeChecker.lifetime) list;
   nf_params         : named_param list;
   nf_ret            : TypeChecker.ty;
   nf_body           : named_expr;
