ocaml/lexer.ml
@@ -39,6 +39,7 @@ let keywords = [
   "true",         Parser.KW_TRUE;
   "false",        Parser.KW_FALSE;
   "bool",         Parser.KW_BOOL;
+  "where",        Parser.KW_WHERE;
 ]
 
 let id_or_kw s =
